src/promotion/SimThreadOther.v
@@ -32,6 +32,37 @@ Require Import SimCommon.
 Set Implicit Arguments.
 
 
+Inductive opt_lang_step: forall (e:ProgramEvent.t) (st1 st2:State.t), Prop :=
+| opt_lang_step_none
+    st:
+    opt_lang_step ProgramEvent.silent st st
+| opt_lang_step_some
+    e st1 st2
+    (STEP: lang.(Language.step) e st1 st2):
+    opt_lang_step e st1 st2
+.
+
+Inductive opt_promise_step: forall (e:ThreadEvent.t) (e1 e2:Thread.t lang), Prop :=
+| opt_promise_step_none
+    e1:
+    opt_promise_step ThreadEvent.silent e1 e1
+| opt_promise_step_some
+    pf e e1 e2
+    (STEP: Thread.promise_step pf e e1 e2):
+    opt_promise_step e e1 e2
+.
+
+Inductive opt_program_step: forall (e:ThreadEvent.t) (e1 e2:Thread.t lang), Prop :=
+| opt_program_step_none
+    e1:
+    opt_program_step ThreadEvent.silent e1 e1
+| opt_program_step_some
+    e e1 e2
+    (STEP: Thread.program_step e e1 e2):
+    opt_program_step e e1 e2
+.
+
+
 Inductive sim_thread_other (l: Loc.t) (e_src e_tgt: Thread.t lang): Prop :=
 | sim_thread_other_intro
     (LOCFREE: loc_free_stmts l e_src.(Thread.state).(State.stmts))
@@ -40,9 +71,38 @@ Inductive sim_thread_other (l: Loc.t) (e_src e_tgt: Thread.t lang): Prop :=
     (SC: sim_timemap l e_src.(Thread.sc) e_tgt.(Thread.sc))
     (MEMORY: sim_memory l e_src.(Thread.memory) e_tgt.(Thread.memory))
     (PROMISES: forall to, Memory.get l to e_src.(Thread.local).(Local.promises) = None)
-    (RELEASED: forall loc from to val released
-                 (GETP: Memory.get loc to e_src.(Thread.local).(Local.promises) =
-                        Some (from, Message.full val (Some released))),
-        released_eq_tview_loc l loc released e_src.(Thread.local).(Local.tview))
 .
 Hint Constructors sim_thread_other.
+
+
+Lemma sim_thread_promise_step
+      l e1_src
+      pf e_tgt e1_tgt e2_tgt
+      (SIM1: sim_thread_other l e1_src e1_tgt)
+      (STEP_TGT: Thread.promise_step pf e_tgt e1_tgt e2_tgt):
+  exists e_src e2_src,
+    <<STEP_SRC: opt_promise_step e_src e1_src e2_src>> /\
+    <<SIM2: sim_thread_other l e2_src e2_tgt>>.
+Proof.
+  inv STEP_TGT. inv LOCAL.
+  destruct (Loc.eq_dec loc l).
+  { subst. esplits; [econs 1|].
+    destruct e1_src. inv SIM1. ss. econs; eauto; ss.
+    - destruct local, lc1. ss.
+      inv LOCAL. econs; eauto. ss.
+      admit.
+    - admit.
+  }
+Admitted.
+
+Lemma sim_thread_step
+      l e1_src
+      pf e_tgt e1_tgt e2_tgt
+      (SIM1: sim_thread_other l e1_src e1_tgt)
+      (STEP_TGT: Thread.step pf e_tgt e1_tgt e2_tgt):
+  exists e_src e2_src,
+    <<STEP_SRC: Thread.opt_step e_src e1_src e2_src>> /\
+    <<SIM2: sim_thread_other l e2_src e2_tgt>> /\
+    <<EVENT: ThreadEvent.get_machine_event e_src = ThreadEvent.get_machine_event e_tgt>>.
+Proof.
+Admitted.
